qc/TImp.v
@@ -1,3 +1,5 @@
+(** * TImp: A Case Study on Typed Imp *)
+
 Set Warnings "-notation-overridden,-parsing".
 Set Warnings "-extraction-opaque-accessed,-extraction".
 Require Import Coq.Bool.Bool.
@@ -13,75 +15,351 @@ Import QcDefaultNotation. Open Scope qc_scope.
 
 Set Bullet Behavior "Strict Subproofs".
 
-Require Import Atom AtomGen Maps QC.
-(* /IMPORTS *)
+Require Import Equalities.
+Require Import QC.
 
-(* The G (option...) monad *)
 
-Definition GOpt A := G (option A).
+(* Leo: Backwards pointer to Imp somehow? *)
+(* Leo: Imp is in the first volume of SF? *)
+(** Having seen a basic overview of QuickChick in the previous chapter, we can
+    now dive into a more realistic case study: a typed variant of Imp.  The
+    original Imp variant presented in the first volume of Software Foundations
+    syntactically separates boolean and arithmetic expressions: [bexp] ranges
+    over boolean expressions, while [aexp] ranges over arithmetic ones.
+    Moreover, variables are only allowed in [aexp] and only take arithmetic
+    values.
+    
+    In typed Imp (TImp) we collapse the expression syntax and allow variables to
+    range over both numbers and booleans. With the unified syntax, we introduce
+    the notion of well-typed Imp expressions and programs: where every variable
+    only ranges over values of a single type throughout the whole program.  We
+    then give an operational semantics to TImp in the form of a partial
+    evaluation function; partial, since in the unified syntax one could attempt
+    to write expressions such as [0 + True].
 
-Instance gOptMonad : `{Monad GOpt} :=
-  {
-    ret A x := returnGen (Some x);
-    bind A B m k := bindGenOpt m k
-  }.
+    A common mantra in functional programming is "well-typed programs cannot go
+    wrong"; TImp is no exception to that rule. The soundness property for TImp
+    will state that evaluating well-typed expressions and programs always
+    succeeds. This is another example of a _conditional_ property. As we saw in
+    the previous chapter, testing such properties requires custom generators.
+    In this chapter, we will show how to scale the techniques for writing
+    generators to more realistic generators for well-typed expressions and
+    programs. In addition, we will also demonstrate the notion and necessity of
+    custom shrinkers preserving invariants, a problem dual to that of custom
+    generators.
+ *)
 
-(* Types *)
+(* ################################################################# *)
+(** * Atoms, Types and Contexts *)
+
+(* ================================================================= *)
+(** ** Atoms *)
+
+(* Leo: How can we cite things in SF-style? *)
+(* Leo: Decide: atoms, [Atom]s or [Atoms]? *)
+(** For the type of identifiers of TImp we are going to borrow (a simplified
+    version of) [Atom] from Penn's Metatheory library. [Atom] is essentially a
+    wrapper around [nat] which supports decidable equality and [fresh]: given
+    any finite set of atoms, one can produce one that is distinct from all of
+    the atoms in the set. 
+  *)
+
+Module Type ATOM <: UsualDecidableType.
+
+  Parameter t : Set.
+  Parameter eq_dec : forall (x y:t), {x = y} + {x <> y}.
+  Parameter fresh : list t -> t.
+  Parameter nat_of: t -> nat.
+
+  Include HasUsualEq <+ UsualIsEq.
+End ATOM.
+
+Module Atom : ATOM.
+
+(** Internally, an [Atom] is just a natural number. *)
+
+  Definition t := nat.
+
+(** Which means decidable equality comes for free from the standard library: *)
+
+  Definition eq_dec := eq_nat_dec.
+  
+(** To compute a fresh natural number given a list of natural numbers,
+    we can just produce the number that is 1 larger than the maximum
+    element: *)
+
+  Fixpoint max_elt (al:list t) : t :=
+    match al with
+      | nil => 0
+      | n'::al' => max n' (max_elt al')
+    end.
+
+  Definition fresh (al:list t) : t :=
+    S (max_elt al).
+
+  Include HasUsualEq <+ UsualIsEq.
+
+(** We also need a way of printing atoms. To support that, we include a 
+    [nat_of] function that exposes the internal natural number. 
+  *)
+  
+  Definition nat_of (a : nat) := a.
+  
+End Atom.
+
+(** We can take advantage of the [nat_of] function of [Atom]s, as well
+    as the [Show] instance of [nat] to print [Atom]s. *)
+
+Instance show_atom : Show Atom.t :=
+  {| show x := show (Atom.nat_of x) |}.
+
+(** To generate identifiers for TImp, we will use a recursive functions 
+    that generates [n] fresh [Atom]s starting from the empty list. *)
+
+Fixpoint get_fresh_atoms n l :=
+  match n with
+  | 0 => l
+  | S n' => get_fresh_atoms n' ((Atom.fresh l) :: l)
+  end.
+
+(* ================================================================= *)
+(** ** Types *)
+
+(** To continue, here is the type of types in TImp, [ty]: *)
 
 Inductive ty := TBool | TNat. 
 
-(* TODO: Actual Generators? Derived? How much have we said at this point? *)
+(** TImp has two types of expressions: booleans and natural numbers. *)
+
+(** As with all user-defined datatypes, in order to use [ty] in testing
+    we will need [Arbitrary], [Show] and an equality [Dec] instance.
+
+    In QC.v, we saw how one can go about writing such generators by hand.
+    However, that process can largely be automated, especially for 
+    simple inductive types (like [ty], [nat], [list], [tree], etc.). 
+    QuickChick provides a top-level vernacular command to derive 
+    such instances. 
+ *)
+
 Derive (Arbitrary, Show) for ty.
+
+(* LEO: Show output? (xxx is defined). Print the derived ones as well? *)
+
+(** The decidable equality instances are not yet derived fully automatically.
+    However, the boilerplate for it is largely straightforward.
+  *)
+
+(* Leo: they've already seen the Dec = boilerplate right? *)
 
 Instance eq_dec_ty (x y : ty) : Dec (x = y).
 Proof. constructor; unfold ssrbool.decidable; decide equality. Defined.
 
+(* ================================================================= *)
+(** ** List Map with Decidable Equality *)
+
+(** To encode typing environments and, later on, states, we will need 
+    maps from atoms to values. The function-based representation in base 
+    Imp is not suited for testing: we will need to be able to access the 
+    domain of the map, fold over it and test for equality; all operations
+    not supported by (Coq) functions. Therefore, we introduce a small 
+    list-based map that takes usual decidable types (like [Atom]) as input.
+
+    The operations we need are:
+    
+       - [empty] : To create the empty map.
+       - [get]   : To look up the binding of an element, if any.
+       - [set]   : To update the binding of an element.
+       - [dom]   : To get the list of keys in the map.
+  *)
+    
+Module Type Map (K:UsualDecidableType).
+
+ Section withv.
+   Variable V : Type.
+    
+   Parameter t : Type -> Type.
+   Parameter empty : t V.
+   Parameter get : t V -> K.t -> option V.
+   Parameter set : t V -> K.t -> V -> t V.
+      Parameter dom : t V -> list K.t.
+       
+    End withv.
+
+End Map.
+
+(** The implementation of the map is a simple association list. 
+    If a list contains multiple tuples with the same key, then 
+    the binding of the key in the map is the one that appears firt 
+    in the list; that is, bindings can be shadowed.
+  *)
+
+Module ListMap (K:UsualDecidableType) <: Map K.
+
+ Section withv.
+   Context {V : Type}.
+    
+   Definition t := list (K.t * V).
+    
+   Definition empty : t := [].
+    
+   Fixpoint get m k : option V := 
+     match m with
+       | [] => None
+       | (k', v) :: m' => if K.eq_dec k k'
+                          then Some v
+                          else get m' k
+     end.
+    
+   Definition set (m:t) (k:K.t) (v:V) : t :=
+     (k, v) :: m.
+    
+   Fixpoint dom (m:t) : list K.t :=
+     match m with
+       | [] => []
+       | (k', v) :: m' => k' :: dom m'
+     end.
+
+ End withv.
+
+End ListMap.
+
+(** We insantiate this functor with [Atom], yielding [AtomMap] our 
+    map with [Atom] as the key type. 
+  *)
+
 Module AtomMap := ListMap (Atom).
+
+(** We introduce a simple inductive proposition, [bind_in m x a], that 
+    holds precisely when the binding of some [Atom] [x] is equal to [a] in 
+    [m] 
+  *)
+
+(* bound_in? *)
+Inductive bind_in {A} : @AtomMap.t A -> Atom.t -> A -> Prop :=
+  | Bind : forall x m a, AtomMap.get m x = Some a -> bind_in m x a.
+
+(** We can now decide whether [bind_in m x a] holds for a given 
+    arrangement of [m], [x] and [a]. In a first reading, you can
+    skip the next few paragraphs that deal with partially automating 
+    the proofs for such instances. 
+  *)
+
+Instance dec_bind_in {A : Type} Gamma x (T : A) 
+         `{D : forall (x y : A), Dec (x = y)}
+  : Dec (bind_in Gamma x T) := {}.
+Proof. 
+  unfold ssrbool.decidable. 
+  destruct (AtomMap.get Gamma x) eqn:Get.
+      
+(** After unfolding [decidable] and destructing [AtomMap.get Gamma x], we are
+    left with two subgoals. In the first, we know that [AtomMap.get Gamma x =
+    Some a] and effectively want to decide whether [AtomMap.get Gamma x = Some
+    T] or not. Which means we need to decide whether [a = T]. Thankfully,
+    we can decide that using our hypothesis [D]. 
+  *)
+  
+  - destruct (D a T) as [[Eq | NEq]]; subst.
+
+(** At this point, the first goal can be immediately decided positevely
+    using constructor. 
+  *)
+
+    + left. constructor. auto.
+
+(** In the second subgoal, we can show that [bind_in] doesn't hold. *)
+
+    + right; intro Contra; inversion Contra; subst; clear Contra.
+      congruence.
+
+(** Both of these tactic patterns are very common in non-trival [Dec] 
+    instances. For that reason, we automate them a bit using LTac.
+  *)
+
+Abort.
+
+(** A lot of the time, we can immediately decide a property positevly 
+    using constructor applications. That is captured in [solve_left]. *)
+
+Ltac solve_left  := try solve [left; econstructor; eauto].
+
+(** Much of the time, we can also immediately decide that a property 
+    doesn't hold by assuming it, doing inversion and using [congruence].
+  *)
+
+Ltac solve_right := 
+  let Contra := fresh "Contra" in
+  try solve [right; intro Contra; inversion Contra; subst; clear Contra; 
+             eauto; congruence].
+
+(** We group both in a single tactic, which does nothing at all if 
+    it fails to solve a goal, thanks to [try solve]. *)
+
+Ltac solve_sum := solve_left; solve_right.
+
+(** We can now prove the [Dec] instance more concisely. *)
+
+Instance dec_bind_in {A : Type} Gamma x (T : A) 
+         `{D : forall (x y : A), Dec (x = y)}
+  : Dec (bind_in Gamma x T) := {}.
+Proof. 
+  unfold ssrbool.decidable. 
+  destruct (AtomMap.get Gamma x) eqn:Get; solve_sum.
+  destruct (D a T) as [[Eq | NEq]]; subst; solve_sum.
+Defined.
+
+(* ================================================================= *)
+(** ** Contexts *)
+
+(** Typing contexts in TImp are just maps from atoms to types. *)
 
 Definition context := @AtomMap.t ty.
 
-(* Wrapper - helpful for automation purposes later *)
-(* bound_in? *)
-Inductive bind_in {A} : @AtomMap.t A -> Atom.t -> A -> Prop :=
-  | Bind : forall x Gamma T, AtomMap.get Gamma x = Some T -> bind_in Gamma x T.
+(** Given a context [Gamma] and a type [T], we can try to generate 
+    a random [Atom] whose binding in [Gamma] is [T]. 
 
-(* Automation stuff for proofs - don't need to show?  Or maybe put it
-   in a magic Tactics.v *)
-Ltac solve_left  := try solve [left; constructor; eauto].
-Ltac solve_right := 
-  let Contra := fresh "Contra" in
-  try solve [right; intro Contra; inversion Contra; subst; clear Contra; eauto; congruence].
-Ltac solve_sum := solve_left; solve_right.
-
-Instance dec_bind_in {A : Type} Gamma x (T : A) `{D : forall (x y : A), Dec (x = y)}
-  : Dec (bind_in Gamma x T).
-Proof. 
-constructor; unfold ssrbool.decidable.
-destruct (AtomMap.get Gamma x) eqn:Get; solve_sum.
-destruct (D a T) eqn:Eq; destruct dec; simpl in *; subst; solve_sum.
-Defined.
-
+    We filter out all of the elements in [Gamma] whose type is
+    equal to [T] and then, for each [(a,T')] that remains we 
+    return the binding [a]. We use the [oneof] combinator to 
+    pick an generator from that list at random. 
+    
+    However, the filtered list might be empty; to facilitate
+    that case, [oneof] also takes a default generator, here [ret None].
+  *)
+    
 Definition gen_typed_atom_from_context (Gamma : context) (T : ty)
                                      : G (option Atom.t) :=
   oneof (ret None) 
-        (List.map (fun '(a,T) => ret (Some a))
+        (List.map (fun '(a,T') => ret (Some a))
                   (List.filter (fun '(a,T') => T = T'?) Gamma)).
 
-(* Hide for lecture? -- explain later *)
-Instance genST_bind_in (Gamma : context) (T : ty) 
-  : GenSuchThat Atom.t (fun x => bind_in Gamma x T) :=
-  { arbitraryST := gen_typed_atom_from_context Gamma T }.
+(** We also need to generate a typing context to begin with. Given 
+    some natural number [n] to serve as the size of the context, 
+    we first create its domain, [n] fresh atoms. 
+    
+    We then create [n] arbitrary types with [vectorOf], using the 
+    [Gen] instance for [ty] we derived earlier.
+  
+    Finally, we zip ([List.combine]) the domain with the ranges and 
+    fold over the resulting, inserting each binding into a map.
+  *)
 
-(* Too many sigs *)
 Definition gen_context (n : nat) : G context := 
   let domain := get_fresh_atoms n [] in
   range <- vectorOf n arbitrary ;;
-  ret (List.fold_left (fun (m : context) (kv : Atom.t * ty) => 
-                         let (k,v) := kv in 
-                         AtomMap.set m k v) 
+  ret (List.fold_left (fun m '(k, v) => AtomMap.set m k v) 
                       (List.combine domain range) AtomMap.empty).
 
-(* Expressions *)
+(* ################################################################# *)
+(** * Expressions *)
+
+(** We are now ready to introduce the syntax of expressions in TImp. 
+    The original Imp had two distinct types of expressions: arithmetic
+    and boolean expressions, while variables were only allowed to 
+    range over natural numbers. In TImp, we extend variables to range 
+    over boolean values as well, collapsing the expressions into a single 
+    type [exp]. 
+
+ *)
 
 Inductive exp : Type :=
   | EVar : Atom.t -> exp
@@ -95,64 +373,236 @@ Inductive exp : Type :=
   | ELe : exp -> exp -> exp
   | ENot : exp -> exp
   | EAnd : exp -> exp -> exp.
+
+(** To be able to print expressions we can derive [Show] *)
+
 Derive Show for exp.
 
-(* Reformat for 70 columns *)
+(** If we tried to derive [Arbitrary] for expressions we would 
+    encounter an error message: 
+    
+    ==> Unable to satisfy the following constraints: 
+        [Gen Atom.t]
+
+    Indeed, we don't have an arbitrary instance for [Atom.t].
+
+  *)
+
+(* EX 3 : Write an instance for [Gen] for [Atom.t], using 
+   [elements] and [get_fresh_atoms]. 
+ *)
+
+(* FILL IN HERE *)   
+
+(* ================================================================= *)
+(** ** Typed Expressions *)
+
+(** The following inductive relation characterizes well-typed expressions
+    of a particular type. It is rather unsurprising, using [bind_in] to 
+    access the typing context in the variable case *)
+
 Inductive has_type : context -> exp -> ty -> Prop := 
-| Ty_Var : forall x T Gamma, bind_in Gamma x T -> has_type Gamma (EVar x) T
-| Ty_Num : forall Gamma n, has_type Gamma (ENum n) TNat
-| Ty_Plus : forall Gamma e1 e2, has_type Gamma e1 TNat -> has_type Gamma e2 TNat ->
-                                has_type Gamma (EPlus e1 e2) TNat
-| Ty_Minus : forall Gamma e1 e2, has_type Gamma e1 TNat -> has_type Gamma e2 TNat ->
-                                has_type Gamma (EMinus e1 e2) TNat
-| Ty_Mult : forall Gamma e1 e2, has_type Gamma e1 TNat -> has_type Gamma e2 TNat ->
-                                has_type Gamma (EMult e1 e2) TNat
-| Ty_True : forall Gamma, has_type Gamma ETrue TBool
-| Ty_False : forall Gamma, has_type Gamma EFalse TBool
-| Ty_Eq : forall Gamma e1 e2, has_type Gamma e1 TNat -> has_type Gamma e2 TNat ->
-                              has_type Gamma (EEq e1 e2) TBool
-| Ty_Le : forall Gamma e1 e2, has_type Gamma e1 TNat -> has_type Gamma e2 TNat ->
-                              has_type Gamma (ELe e1 e2) TBool
-| Ty_Not : forall Gamma e, has_type Gamma e TBool ->
-                              has_type Gamma (ENot e) TBool
-| Ty_And : forall Gamma e1 e2, has_type Gamma e1 TBool -> has_type Gamma e2 TBool ->
-                               has_type Gamma (EAnd e1 e2) TBool.
+| Ty_Var : forall x T Gamma, 
+    bind_in Gamma x T -> 
+    has_type Gamma (EVar x) T
+| Ty_Num : forall Gamma n, 
+    has_type Gamma (ENum n) TNat
+| Ty_Plus : forall Gamma e1 e2, 
+    has_type Gamma e1 TNat -> has_type Gamma e2 TNat ->
+    has_type Gamma (EPlus e1 e2) TNat
+| Ty_Minus : forall Gamma e1 e2, 
+    has_type Gamma e1 TNat -> has_type Gamma e2 TNat ->
+    has_type Gamma (EMinus e1 e2) TNat
+| Ty_Mult : forall Gamma e1 e2, 
+    has_type Gamma e1 TNat -> has_type Gamma e2 TNat ->
+    has_type Gamma (EMult e1 e2) TNat
+| Ty_True : forall Gamma, 
+    has_type Gamma ETrue TBool
+| Ty_False : forall Gamma, 
+    has_type Gamma EFalse TBool
+| Ty_Eq : forall Gamma e1 e2, 
+    has_type Gamma e1 TNat -> has_type Gamma e2 TNat ->
+    has_type Gamma (EEq e1 e2) TBool
+| Ty_Le : forall Gamma e1 e2, 
+    has_type Gamma e1 TNat -> has_type Gamma e2 TNat ->
+    has_type Gamma (ELe e1 e2) TBool
+| Ty_Not : forall Gamma e, 
+    has_type Gamma e TBool ->
+    has_type Gamma (ENot e) TBool
+| Ty_And : forall Gamma e1 e2, 
+    has_type Gamma e1 TBool -> has_type Gamma e2 TBool ->
+    has_type Gamma (EAnd e1 e2) TBool.
 
-(* Show this later *)
-Derive ArbitrarySizedSuchThat for (fun e => has_type Gamma e T).
+(* Move to Tactics.v *)
+Ltac solve_inductives Gamma :=
+  repeat (match goal with 
+      [ IH : forall _ _, _ |- _ ] =>
+      let H1 := fresh "H1" in 
+      pose proof (IH TNat Gamma) as H1;
+      let H2 := fresh "H2" in 
+      pose proof (IH TBool Gamma) as H2;
+      clear IH;
+      destruct H1; destruct H2; solve_sum
+    end).
 
-(* This is so pedantic I want to derive it :) *)
-Fixpoint gen_exp_typed_sized (size : nat) (Gamma : context) (T : ty) : G (option exp) :=
-  let gen_typed_evar : G (option exp) := 
-      x <- gen_typed_atom_from_context Gamma T;;
-      ret (EVar x) in
-  let base :=
-      (2, gen_typed_evar) ::
+(** Typing in TImp is decidable: given an expression [e], a context [Gamma] 
+    and a type [T], we can decide whether [has_type Gamma e T] holds. 
+    We implement that in a [Dec] instance. *)
+
+Instance dec_has_type (e : exp) (Gamma : context) (T : ty) 
+  : Dec (has_type Gamma e T) :=
+  { dec := _ }.
+Proof with solve_sum.
+  (* I need move: *)
+  generalize dependent Gamma.
+  generalize dependent T.
+  induction e; intros T Gamma; unfold ssrbool.decidable;
+    try solve [destruct T; solve_sum];
+    try solve [destruct T; solve_inductives Gamma].
+  (* bind_in case *)
+  destruct (dec_bind_in Gamma t T); destruct dec; solve_sum.
+Defined.
+
+(* EX 4 : Derive [Arbitrary] for expressions and write a conditional 
+    property that is always true, if an expression is well-typed. Try to 
+    check that property. What happens?  
+
+    (You will need to provide a [Shrink] instance for [Atom]. The
+    result of shrinking an atom can be empty for now)
+  *)
+
+(* FILL IN HERE *)
+
+(* ================================================================= *)
+(** ** Generator for Typed expressions *)
+
+(** Instead of generating expressions and filtering them using 
+    has_type, we can be smarter and generate well typed expressions 
+    for a given context directly. It is common for conditional generators 
+    to return [option]s of the underlying type, allowing the possibility of 
+    failure if a wrong choice is made. For example, if we wanted to generate
+    an expression of type [TNat] and chose to do that by generating a variable, 
+    then we might not be able to actually do that (e.g. if the context is empty). 
+   
+*)
+
+(** To chain two different generetors with type [G (option A)], we need to 
+    execute the first generator, match on its result, and, when it is a [Some], 
+    apply the second generator.
+  *)
+
+Definition bindGenOpt {A B : Type} (gma : G (option A)) (k : A -> G (option B)) 
+  : G (option B) :=
+  ma <- gma ;;
+  match ma with 
+  | Some a => k a 
+  | None => ret None
+  end.
+
+(** This pattern is common enough that QuickChick provides explicit monadic 
+    notation support *)
+
+Definition GOpt A := G (option A).
+
+Instance gOptMonad : `{Monad GOpt} :=
+  {
+    ret A x := returnGen (Some x);
+    bind A B m k := bindGenOpt m k
+  }.
+
+(** Which brings us to our first large sized generator for typed expressions.
+    We asumme that [Gamma] and [T] are inputs to the generation process. We also
+    use a [size] parameter to control the depth of generated expressions.
+
+    For the shape of the generator we turn to [has_type], the relation we are
+    trying to satisfy. First of all, we need to identify which cases can be
+    "base cases" and which need to be recursive. In the case of has_type,
+    [Ty_Var], [Ty_Num], [Ty_True] and [Ty_False] are the only cases where
+    [has_type] doesn't appear as a side-condition, and are therefore
+    base cases.
+
+    We will use the [backtrack] combinator
+
+      [ backtrack : list (nat * G (option ?A)) -> G (option ?A) ]
+
+    which operates similarly to frequency for optional generators. 
+    However, unlike frequency, if the generator that was selected 
+    first fails (returns [None]), then [backtrack] proceeds to pick
+    one of the remaining ones until it runs out or one succeeds. 
+
+  *)
+
+(** We will break the generator into smaller bits.
+    
+    Let's start with the first derivation of [has_type], [Ty_Var].
+
+    [Ty_Var : forall (x : Atom.t) (T : ty) (Gamma : AtomMap.t),
+              bind_in Gamma x T -> has_type Gamma (EVar x) T]
+
+    Since we want to generate expressions such that [has_type Gamma e T] holds given [Gamma] and [T], following this rule we would need to generate 
+    an expression of the form [EVar x] for some atom [x]. The side 
+    condition [bind_in Gamma x T] informs what that atom must be: it must 
+    be an [Atom] from the context with the appropriate type. That's exactly
+    what [gen_typed_atom_from_context] did.
+
+  *)
+
+Definition gen_typed_evar (Gamma : context) (T : ty) : G (option exp) :=
+  x <- gen_typed_atom_from_context Gamma T;;
+  ret (EVar x).
+
+(** For the rest of the base cases, we need to pattern match on the 
+    input type [T]: if it is [TNat], then we need to generate an arbitrary 
+    integer [n] and wrap it in an [ENum]; if it is [TBool], we need to pick 
+    between [ETrue] and [EFalse]. 
+   
+    Since [base] will be the input to [backtrack], we need to add natural numbers 
+    as weights. Since this example is simple enough, we selected [1] for 
+    all weights. In larger applications, we would need to fine tune these 
+    weights to obtain a desired distribution. 
+  *)
+
+Definition base Gamma T := 
+      (2, gen_typed_evar Gamma T) ::
       match T with 
       | TNat  => [ (2, n <- arbitrary;; ret (Some (ENum n)))]
       | TBool => [ (1, ret ETrue)
                  ; (1, ret EFalse) ]
-      end in 
+      end.
+
+(** In the recursive branches, we also need to pattern match on [T]. 
+    If, for example, [T = TNat], then we can only satisfy typing 
+    derivations whose conclusion is of the form [has_type Gamma _ TNat], 
+    i.e. [Ty_Plus], [Ty_Minus] and [Ty_Mult]. 
+
+    Consider [Ty_Plus]: we will need to recursively generate 
+    expressions [e1] and [e2] that have type [TNat], with potentially smaller 
+    sizes to ensure termination. 
+
+    We put everything together in the following generator *)
+
+Fixpoint gen_exp_typed_sized (size : nat) (Gamma : context) (T : ty) : G (option exp) :=
+  let base := base Gamma T in
   let recs size' := 
       match T with 
-      | TNat => [ (1, e1 <- gen_exp_typed_sized size' Gamma TNat ;; 
+      | TNat => [ (size, e1 <- gen_exp_typed_sized size' Gamma TNat ;; 
                       e2 <- gen_exp_typed_sized size' Gamma TNat ;; 
                       ret (EPlus e1 e2)) 
-                ; (1, e1 <- gen_exp_typed_sized size' Gamma TNat ;; 
+                ; (size, e1 <- gen_exp_typed_sized size' Gamma TNat ;; 
                       e2 <- gen_exp_typed_sized size' Gamma TNat ;; 
                       ret (EMinus e1 e2)) 
-                ; (1, e1 <- gen_exp_typed_sized size' Gamma TNat ;; 
+                ; (size, e1 <- gen_exp_typed_sized size' Gamma TNat ;; 
                       e2 <- gen_exp_typed_sized size' Gamma TNat ;; 
                       ret (EMult e1 e2)) ]
-      | TBool => [ (1, e1 <- gen_exp_typed_sized size' Gamma TNat ;; 
+      | TBool => [ (size, e1 <- gen_exp_typed_sized size' Gamma TNat ;; 
                        e2 <- gen_exp_typed_sized size' Gamma TNat ;; 
                        ret (EEq e1 e2)) 
-                 ; (1, e1 <- gen_exp_typed_sized size' Gamma TNat ;; 
+                 ; (size, e1 <- gen_exp_typed_sized size' Gamma TNat ;; 
                        e2 <- gen_exp_typed_sized size' Gamma TNat ;; 
                        ret (ELe e1 e2)) 
-                 ; (1, e1 <- gen_exp_typed_sized size' Gamma TBool ;; 
+                 ; (size, e1 <- gen_exp_typed_sized size' Gamma TBool ;; 
                        ret (ENot e1))
-                 ; (1, e1 <- gen_exp_typed_sized size' Gamma TBool ;; 
+                 ; (size, e1 <- gen_exp_typed_sized size' Gamma TBool ;; 
                        e2 <- gen_exp_typed_sized size' Gamma TBool ;; 
                        ret (EAnd e1 e2)) ]
       end in
@@ -163,7 +613,216 @@ Fixpoint gen_exp_typed_sized (size : nat) (Gamma : context) (T : ty) : G (option
     backtrack (base ++ recs size')
   end.
 
-(* Move to after the first bug *)
+(** When writing such complex generators, it's good to have small tests 
+    that ensure that you are generating what you expect. For example, we 
+    would expect [gen_exp_typed_sized] to always return expressions that are 
+    well typed. 
+    
+    We can use [forAll] to encode such a property. 
+  *)
+
+Definition gen_typed_has_type :=
+  let num_vars := 4 in
+  let top_level_size := 3 in 
+  forAll (gen_context num_vars) (fun Gamma =>
+  forAll arbitrary (fun T =>                                   
+  forAll (gen_exp_typed_sized top_level_size Gamma T) (fun me =>
+  match me with 
+  | Some e => (has_type Gamma e T)?
+  | _ => false (* this should NEVER fail *)
+  end))).
+
+(* QuickChick gen_typed_has_type. *)
+
+(* ################################################################# *)
+(** * Values and States *)
+
+(* ================================================================= *)
+(** ** Values *)
+
+(** In original Imp, variables range over natural numbers, so states were just
+    maps from identifiers to [nat]. Since we wanted to extend this to also 
+    include booleans, we introduce the type of [value]s which includes both. 
+  *)
+
+
+Inductive value := VNat : nat -> value | VBool : bool -> value.
+
+Derive Show for value.
+
+(** We can also quickly define a typing relation for values, a Dec instance
+    for it and a generator for values of a given type. *)
+  
+Inductive has_type_value : value -> ty -> Prop :=
+  | TyVNat  : forall n, has_type_value (VNat  n) TNat
+  | TyVBool : forall b, has_type_value (VBool b) TBool.
+
+Instance dec_has_type_value v T : Dec (has_type_value v T).
+Proof. constructor; unfold ssrbool.decidable.
+destruct v; destruct T; solve_sum.
+Defined.
+
+Definition gen_typed_value (T : ty) : G value :=
+  match T with 
+  | TNat  => n <- arbitrary;; ret (VNat n)
+  | TBool => b <- arbitrary;; ret (VBool b)
+  end.
+
+(* ================================================================= *)
+(** ** States *)
+
+(** States in TImp are just maps from atoms to values *)
+
+Definition state := @AtomMap.t value.
+
+(** We introduce an inductive relation that specifies when a state
+    is well-typed according to a context: that is, when all of 
+    its variables are mapped to values of appropriate types. 
+  
+    We encode this in an element-by-element style inductive relation: 
+    empty states are only well-typed with respect to an empty context, 
+    while non-empty states need to map their head atom to a value of the 
+    appropriate type and their tails must also be well typed.
+  *)
+
+Inductive typed_state : context -> state -> Prop :=
+| TS_Empty : typed_state AtomMap.empty AtomMap.empty
+| TS_Elem  : forall x v T st Gamma, 
+    has_type_value v T -> typed_state Gamma st ->
+    typed_state ((x,T)::Gamma) ((x,v)::st).
+
+Instance dec_typed_state Gamma st : Dec (typed_state Gamma st).
+Proof. 
+constructor; unfold ssrbool.decidable.
+generalize dependent Gamma.
+induction st; intros; destruct Gamma; solve_sum.
+destruct a as [a v]; destruct p as [a' T].
+destruct (Atom.eq_dec a a'); solve_sum.
+subst; specialize (IHst Gamma); destruct IHst; solve_sum.
+destruct (dec_has_type_value v T); destruct dec; solve_sum.
+Defined.
+
+(** To write a generator for well typed states given a context [Gamma], 
+    we use the combinator [sequenceGen : list (G A) -> G (list A)], that 
+    receives a list of generators and produces a generator of lists. 
+    This is what Haskell's [sequence] combinator would do for the monad [G]. 
+  
+    We just need to iterate ([map]) through the context, producing
+    an arbitrary value of the appropriate type for each pair [(x,T)]. The 
+    [sequenceGen] combinator will then chain all those generators in sequence,
+    producing a generator for well-typed states *)
+    
+
+Definition gen_typed_state (Gamma : context) : G state := 
+  sequenceGen (List.map (fun '(x, T) =>
+                           v <- gen_typed_value T;;
+                           ret (x, v)) Gamma).
+
+
+(* ################################################################# *)
+(** * Evaluation *)
+
+(** Our evaluation function, takes a state and an expression and returns 
+    an optional value, assuming that the expression has a type 
+    with respect to the state. 
+  *)
+
+Fixpoint eval (st : state) (e : exp) : option value :=
+  match e with
+  | EVar x => AtomMap.get st x
+  | ENum n => Some (VNat n)
+  | EPlus e1 e2 => 
+    match eval st e1, eval st e2 with 
+    | Some (VNat n1), Some (VNat n2) => Some (VNat (n1 + n2))
+    | _, _ => None
+    end 
+  | EMinus e1 e2 => 
+    match eval st e1, eval st e2 with 
+    | Some (VNat n1), Some (VNat n2) => Some (VNat (n1 - n2))
+    | _, _ => None
+    end
+  | EMult e1 e2 => 
+    match eval st e1, eval st e2 with 
+    | Some (VNat n1), Some (VNat n2) => Some (VNat (n1 * n2))
+    | _, _ => None
+    end
+  | ETrue       => Some (VBool true  )
+  | EFalse      => Some (VBool false )
+  | EEq e1 e2 => 
+    match eval st e1, eval st e2 with 
+    | Some (VNat n1), Some (VNat n2) => Some (VBool (n1 =? n2))
+    | _, _ => None
+    end
+  | ELe e1 e2 => 
+    match eval st e1, eval st e2 with 
+    | Some (VNat n1), Some (VNat n2) => Some (VBool (n1 <? n2))
+    | _, _ => None
+    end
+  | ENot e => 
+    match eval st e with 
+    | Some (VBool b) => Some (VBool (negb b))
+    | _ => None
+    end
+  | EAnd e1 e2  => 
+    match eval st e1, eval st e2 with 
+(* Leo: Stupidest bug possible *)
+    | Some (VBool b), Some (VNat n2) => Some (VBool (negb b))
+(*    | Some (VBool b1), Some (VBool b2) => Some (VBool (andb b1 b2)) *)
+    | _, _ => None
+    end
+  end.
+
+(** Type Soundness states that if we have an expression [e] of a given type [T], 
+    as well as a well-typed state [st], then evaluating [e] in [st] will
+    never fail.*)
+
+Definition isNone {A : Type} (m : option A) :=
+  match m with 
+  | None => true
+  | _ => false
+  end.
+
+Conjecture expression_soundness : 
+  forall Gamma st e T,
+    typed_state Gamma st ->
+    has_type Gamma e T ->
+    isNone (eval st e) = false.
+
+(** To test that property, we construct an appropriate checker *)
+
+Definition expression_soundness_exec := 
+  let num_vars := 4 in 
+  let top_level_size := 3 in
+  forAll (gen_context num_vars)  (fun Gamma =>
+  forAll (gen_typed_state Gamma) (fun st =>
+  forAll arbitrary (fun T =>                                    
+  forAll (gen_exp_typed_sized 3 Gamma T) (fun me => 
+  match me with  
+  | Some e => negb (isNone (eval st e))
+  | _ => false
+  end)))).   
+
+(* QuickChick expression_soundness_exec. *)
+
+(** But where is the bug? :o 
+    We need shrinking. *)
+
+(* ================================================================= *)
+(** ** Shrinking for Expressions *)
+
+(** We not only need to shrink expressions, we need to shrink them 
+    so that their type is preserved! To accomplish that we need to follow 
+    a reverse procedure than with the generators: look at a typing derivation
+    and see what parts of it we can shrink to appropriate types so that 
+    the entire thing is preserved.
+   
+    For example, to shrink [EPlus e1 e2], we could shrink [e1] or [e2] preserving 
+    their [TNat] type, or shrink to [e1] or [e2] themselves. However, for 
+    [EEq e1 e2], we could to shrink [e1] or [e2] again preserving their [TNat]
+    types, but we couldn't shrink to [e1] or [e2] as their type is wrong. 
+ *)
+   
+
 Fixpoint shrink_exp_typed (T : ty) (e : exp) : list exp :=
   match e with 
   | EVar _ => 
@@ -202,48 +861,10 @@ Fixpoint shrink_exp_typed (T : ty) (e : exp) : list exp :=
        ++ (List.map (fun e2' => EAnd e1 e2') (shrink_exp_typed TBool e2))
   end.
 
-(* Move to Tactics.v *)
-Ltac solve_inductives Gamma :=
-  repeat (match goal with 
-      [ IH : forall _ _, _ |- _ ] =>
-      let H1 := fresh "H1" in 
-      pose proof (IH TNat Gamma) as H1;
-      let H2 := fresh "H2" in 
-      pose proof (IH TBool Gamma) as H2;
-      clear IH;
-      destruct H1; destruct H2; solve_sum
-    end).
-
-(* Too much automation? *)
-Instance dec_has_type (e : exp) (Gamma : context) (T : ty) : Dec (has_type Gamma e T) :=
-  { dec := _ }.
-Proof with solve_sum.
-  (* I need move: *)
-  generalize dependent Gamma.
-  generalize dependent T.
-  induction e; intros T Gamma; unfold ssrbool.decidable;
-    try solve [destruct T; solve_sum];
-    try solve [destruct T; solve_inductives Gamma].
-  (* bind_in case *)
-  destruct (dec_bind_in Gamma t T); destruct dec; solve_sum.
-Defined.
-
-(* Sanity checks *)
-(* Generation sanity check *)
-Definition gen_typed_has_type :=
-  let num_vars := 4 in
-  let top_level_size := 3 in 
-  forAll (gen_context num_vars) (fun Gamma =>
-  forAll arbitrary (fun T =>                                   
-  forAll (gen_exp_typed_sized top_level_size Gamma T) (fun me =>
-  match me with 
-  | Some e => (has_type Gamma e T)?
-  | _ => false (* this should NEVER fail *)
-  end))).
-
-(* QuickChick gen_typed_has_type. *)
-
-(* Shrinking sanity check *)
+(** Similarly with generators, we can have a sanity check for our shrinking:
+    Given a random expression of a given type, all of the results of [shrink]
+    should have the same type. *)
+    
 Definition shrink_typed_has_type :=
   let num_vars := 4 in
   let top_level_size := 3 in 
@@ -258,112 +879,11 @@ Definition shrink_typed_has_type :=
 
 (* QuickChick shrink_typed_has_type. *)
 
-Inductive value := VNat : nat -> value | VBool : bool -> value.
+(* ================================================================= *)
+(** ** Back to soundness *)
 
-Derive Show for value.
-  
-Inductive has_type_value : value -> ty -> Prop :=
-  | TyVNat  : forall n, has_type_value (VNat  n) TNat
-  | TyVBool : forall b, has_type_value (VBool b) TBool.
-
-Instance dec_has_type_value v T : Dec (has_type_value v T).
-Proof. constructor; unfold ssrbool.decidable.
-destruct v; destruct T; solve_sum.
-Defined.
-
-Definition gen_typed_value (T : ty) : G value :=
-  match T with 
-  | TNat  => n <- arbitrary;; ret (VNat n)
-  | TBool => b <- arbitrary;; ret (VBool b)
-  end.
-
-Definition state := @AtomMap.t value.
-
-(* Similar structure *)
-Inductive typed_state : context -> state -> Prop :=
-| TS_Empty : typed_state AtomMap.empty AtomMap.empty
-| TS_Elem  : forall x v T st Gamma, 
-    has_type_value v T -> typed_state Gamma st ->
-    typed_state ((x,T)::Gamma) ((x,v)::st).
-
-Instance dec_typed_state Gamma st : Dec (typed_state Gamma st).
-(* TODO: Fold all such stuff, like this: *)
-Proof. 
-constructor; unfold ssrbool.decidable.
-generalize dependent Gamma.
-induction st; intros; destruct Gamma; solve_sum.
-destruct a as [a v]; destruct p as [a' T].
-destruct (Atom.eq_dec a a'); solve_sum.
-subst; specialize (IHst Gamma); destruct IHst; solve_sum.
-destruct (dec_has_type_value v T); destruct dec; solve_sum.
-Defined.
-
-Definition gen_typed_state (Gamma : context) : G state := 
-  sequenceGen (List.map (fun '(x, T) =>
-                           v <- gen_typed_value T;;
-                           ret (x, v)) Gamma).
-(* Use typeclasses? *)
-
-Instance genST_typed_state (Gamma : context) : 
-  GenSuchThat state (fun st => typed_state Gamma st) :=
-  { arbitraryST := liftGen Some (gen_typed_state Gamma) }.
-
-(* Monadify *)
-Fixpoint eval (st : state) (e : exp) : option value :=
-  match e with
-  | EVar x => AtomMap.get st x
-  | ENum n => Some (VNat n)
-  | EPlus e1 e2 => 
-    match eval st e1, eval st e2 with 
-    | Some (VNat n1), Some (VNat n2) => Some (VNat (n1 + n2))
-    | _, _ => None
-    end
-  | EMinus e1 e2 => 
-    match eval st e1, eval st e2 with 
-    | Some (VNat n1), Some (VNat n2) => Some (VNat (n1 - n2))
-    | _, _ => None
-    end
-  | EMult e1 e2 => 
-    match eval st e1, eval st e2 with 
-    | Some (VNat n1), Some (VNat n2) => Some (VNat (n1 * n2))
-    | _, _ => None
-    end
-  | ETrue       => Some (VBool true  )
-  | EFalse      => Some (VBool false )
-  | EEq e1 e2 => 
-    match eval st e1, eval st e2 with 
-    | Some (VNat n1), Some (VNat n2) => Some (VBool (n1 =? n2))
-    | _, _ => None
-    end
-  | ELe e1 e2 => 
-    match eval st e1, eval st e2 with 
-    | Some (VNat n1), Some (VNat n2) => Some (VBool (n1 <? n2))
-    | _, _ => None
-    end
-  | ENot e => 
-    match eval st e with 
-    | Some (VBool b) => Some (VBool (negb b))
-    | _ => None
-    end
-  | EAnd e1 e2  => 
-    match eval st e1, eval st e2 with 
-    | Some (VBool b1), Some (VBool b2) => Some (VBool (andb b1 b2))
-    | _, _ => None
-    end
-  end.
-
-Definition isNone {A : Type} (m : option A) :=
-  match m with 
-  | None => true
-  | _ => false
-  end.
-
-(* Soundness for expressions *)
-Conjecture expression_soundness : 
-  forall Gamma st e T,
-    typed_state Gamma st ->
-    has_type Gamma e T ->
-    isNone (eval st e) = false.
+(** To lift the shrinker to optional expressions, QuickChick provides a [lift]
+    function. *)
 
 Definition lift_shrink {A : Type} (shr : A -> list A) (m : option A) : list (option A) :=
   match m with 
@@ -371,26 +891,27 @@ Definition lift_shrink {A : Type} (shr : A -> list A) (m : option A) : list (opt
   | _ => []
   end.
 
-Definition expression_soundness_exec := 
+(** Armed with shrinking we can pinpoint the bug in the [EAnd] branch 
+    and remove the obvious bug. *)
+
+Definition expression_soundness_exec' := 
   let num_vars := 4 in 
   let top_level_size := 3 in
   forAll (gen_context num_vars)  (fun Gamma =>
   forAll (gen_typed_state Gamma) (fun st =>
   forAll arbitrary (fun T =>                                    
-  forAllShrink (gen_exp_typed_sized 3 Gamma T) (lift_shrink (shrink_exp_typed T)) (fun me => 
-  match me with 
+  forAllShrink (gen_exp_typed_sized 3 Gamma T) (lift_shrink (shrink_exp_typed T)) (fun me =>  
+  match me with  
   | Some e => negb (isNone (eval st e))
   | _ => false
   end)))).   
 
-(* QuickChick expression_soundness_exec. *)
-(* Try adding a bug and see if we can find it
+(* QuickChick expression_soundness_exec'. *)
 
-Do it first with forAll, not forAllShrink, then observe that the bug
-is hard to see.  Show shrinking, redo the property,  *)
+(* ################################################################# *)
+(** * Well-typed programs *)
 
-
-(* Start exercise here *)
+(** We now introduce TImp commands, exactly like the ones in Imp *)
 
 Inductive com : Type :=
   | CSkip  : com
@@ -418,55 +939,89 @@ Notation "'WHILE' b 'DO' c 'END'" :=
 Notation "'IFB' c1 'THEN' c2 'ELSE' c3 'FI'" :=
   (CIf c1 c2 c3) (at level 80, right associativity).
 
-(* This is so pedantic I want to derive it :) *)
-Fixpoint gen_com_typed_sized (size : nat) (Gamma : context) : G (option com) :=
-  let assgn := 
-                (List.map (fun '(x,T) =>
-                             (1, e <- gen_exp_typed_sized size Gamma T;;
-                                ret (CAss x e)))
-                          Gamma)
-  in 
-  let skip :=
-      ret SKIP in
-  let recs size' := 
-      [ (1, c1 <- gen_com_typed_sized size' Gamma;;
-            c2 <- gen_com_typed_sized size' Gamma;;
-            ret (CSeq c1 c2))
-      ; (1, c <- gen_com_typed_sized size' Gamma;;
-            b <- gen_exp_typed_sized size' Gamma TBool;;
-            ret (CWhile b c))
-      ; (1, b <- gen_exp_typed_sized size' Gamma TBool;;
-            c1 <- gen_com_typed_sized size' Gamma;;
-            c2 <- gen_com_typed_sized size' Gamma;;
-            ret (CIf b c1 c2))
-      ] in
-  match size with 
-  | O => backtrack ((1, skip) :: assgn)
-  | S size' => backtrack ((1, skip) :: (assgn ++ recs size'))
+(* ================================================================= *)
+(** ** Well-typed commands *)
+
+Inductive well_typed_com : context -> com -> Prop :=
+  | TSkip : forall Gamma, well_typed_com Gamma CSkip
+  | TAss  : forall Gamma x e T, 
+      bind_in Gamma x T -> has_type Gamma e T ->
+      well_typed_com Gamma (CAss x e)
+  | TSeq  : forall Gamma c1 c2, 
+      well_typed_com Gamma c1 -> well_typed_com Gamma c2 ->
+      well_typed_com Gamma (CSeq c1 c2)
+  | TIf : forall Gamma b c1 c2, 
+      has_type Gamma b TBool ->
+      well_typed_com Gamma c1 -> well_typed_com Gamma c2 ->
+      well_typed_com Gamma (CIf b c1 c2)
+  | TWhile : forall Gamma b c,
+      has_type Gamma b TBool -> well_typed_com Gamma c -> 
+      well_typed_com Gamma (CWhile b c).
+
+(** Decidable instance for well-typed *)
+
+(** A couple of theorems to help the decidability proof *)
+
+Theorem bind_deterministic Gamma x (T1 T2 : ty) :
+  bind_in Gamma x T1 -> bind_in Gamma x T2 -> 
+  T1 = T2.
+Proof.
+  destruct T1; destruct T2; intros H1 H2; eauto; 
+    inversion H1; inversion H2; congruence.
+Qed.
+
+Theorem has_type_deterministic Gamma e (T1 T2 : ty) : 
+  has_type e Gamma T1 -> has_type e Gamma T2 -> 
+  T1 = T2.
+Proof.
+  destruct T1; destruct T2; intros H1 H2; eauto;
+    inversion H1; inversion H2; subst; eauto; try congruence;
+  inversion H7; subst;
+    eapply bind_deterministic; eauto.
+Qed.
+
+(* More tactic magic *)
+Ltac solve_det := 
+  match goal with 
+  | [ H1 : bind_in _ _ ?T1 ,
+      H2 : bind_in _ _ ?T2 |- _ ] =>
+    assert (T1 = T2) by (eapply bind_deterministic; eauto)
+  | [ H1 : has_type _ _ ?T1 ,
+      H2 : has_type _ _ ?T2 |- _ ] =>
+    assert (T1 = T2) by (eapply bind_deterministic; eauto)
   end.
 
-Fixpoint shrink_com_typed (Gamma : context) (c : com) : list com := 
-  match c with 
-  | SKIP => []
-  | CAss x e => 
-    match AtomMap.get Gamma x with
-    | Some T => SKIP :: List.map (fun e' => CAss x e) (shrink_exp_typed T e)
-    | _ => []
-    end
-  | CSeq c1 c2 =>
-    c1 :: c2 
-       :: (List.map (fun c1' => CSeq c1' c2) (shrink_com_typed Gamma c1))
-       ++ (List.map (fun c2' => CSeq c1 c2') (shrink_com_typed Gamma c2))
-  | CIf b c1 c2 =>
-    c1 :: c2 
-       :: (List.map (fun c1' => CIf b c1' c2) (shrink_com_typed Gamma c1))
-       ++ (List.map (fun c2' => CIf b c1 c2') (shrink_com_typed Gamma c2))
-       ++ (List.map (fun b' => CIf b' c1 c2) (shrink_exp_typed TBool b))
-  | CWhile b c =>
-    c :: (CIf b c c) 
-      :: (List.map (fun b' => CWhile b' c) (shrink_exp_typed TBool b))
-      ++ (List.map (fun c' => CWhile b c') (shrink_com_typed Gamma c))
-  end.
+(* We also provide a (brute-force) decidability procedure for well typed 
+   programs *)
+Instance dec_well_typed_com (Gamma : context) (c : com) : Dec (well_typed_com Gamma c) := {}.
+Proof with eauto.
+  unfold ssrbool.decidable.
+  induction c; solve_sum.
+  - destruct (dec_bind_in Gamma t TNat); destruct dec;
+    destruct (dec_has_type e Gamma TNat); destruct dec; 
+    destruct (dec_bind_in Gamma t TBool); destruct dec;
+    destruct (dec_has_type e Gamma TBool); destruct dec; solve_sum;
+    try solve_det; try congruence;
+    right; intro Contra; inversion Contra; subst; clear Contra;
+    try solve_det; try congruence;
+    destruct T; eauto.
+  - destruct IHc1; destruct IHc2; subst; eauto; solve_sum.
+  - destruct IHc1; destruct IHc2; subst; eauto; solve_sum.
+    destruct (dec_has_type e Gamma TBool); destruct dec; solve_sum.
+  - destruct IHc; 
+    destruct (dec_has_type e Gamma TBool); destruct dec; solve_sum.
+Qed.
+
+(** Exercise 4 : Write a generator and a shrinker for well_typed programs
+    given some context [Gamma]. Write sanity checks to check your work. *)
+
+(* FILL IN HERE *)
+
+(** To complete the tour of TImp, here is a (buggy?) evaluation function for 
+    commands given a state. To ensure termination, we include an 
+    additional fuel parameter: if that runs out we return [OutOfGas], signifying  
+    that we're not sure if evaluation would have succeeded or failed later. 
+  *)
   
 Inductive result := 
 | Success : state -> result
@@ -490,9 +1045,9 @@ Fixpoint ceval (fuel : nat) (st : state) (c : com) : result :=
         match ceval fuel' st c1 with 
         | Success st' =>  ceval fuel' st' c2 
         (* Bug : On OutOfGas should out of Gas :
-        | _ => Fail 
-        *)
         | r => r
+        *)
+        | _ => Fail 
         end
     | IFB b THEN c1 ELSE c2 FI =>
       match eval st b with 
@@ -515,52 +1070,14 @@ Definition isFail r :=
   | _ => false
   end.
 
+(** Our type soundness property is that well_typed commands never fail *)
 Conjecture well_typed_state_never_stuck : 
   forall Gamma st, typed_state Gamma st ->
-  forall fuel c, isFail (ceval fuel st c) = false.
+  forall c, well_typed_com Gamma c ->
+  forall fuel, isFail (ceval fuel st c) = false.
 
-Definition well_typed_state_never_stuck_exec := 
-  let num_vars := 4 in 
-  let top_level_size := 5 in
-  forAll (gen_context num_vars)  (fun Gamma =>
-  forAll (gen_typed_state Gamma) (fun st =>
-  forAllShrink arbitrary shrink (fun fuel =>
-  forAllShrink (gen_com_typed_sized 3 Gamma) (lift_shrink (shrink_com_typed Gamma)) (fun mc => 
-  match mc with 
-  | Some c => negb (isFail (ceval fuel st c))
-  | _ => false
-  end)))).                      
+(* Exercise 4: Write a checker for the above property, find any bugs 
+   and fix them *)
 
-(* QuickChick well_typed_state_never_stuck_exec. *)
-  
-(* Unreadable bug? 
-QuickChecking well_typed_state_never_stuck_exec
-[(1,TBool), (2,TBool), (3,TNat), (4,TBool)]
-[(1,VBool false), (2,VBool false), (3,VNat 5), (4,VBool true)]
-6
-Some CWhile (EAnd (EEq (EPlus (ENum 2) (ENum 3)) (ENum 5)) (ENot EFalse)) (CIf (ELe (EMinus (ENum 2) (EMinus (EVar 3) (EVar 3))) (ENum 1)) (CAss 1 (EVar 4)) (CAss 2 (EVar 1)))
-*** Failed after 7 tests and 0 shrinks
-*)
+(* FILL IN HERE *)                  
 
-(* Really motivates shrinking... 
-QuickChecking well_typed_state_never_stuck_exec
-[(1,TBool), (2,TBool), (3,TNat), (4,TBool)]
-[(1,VBool false), (2,VBool true), (3,VNat 0), (4,VBool false)]
-1
-Some CSeq CSkip CSkip
-*)
-
-(* LEO: Fix in SF: it should be c ;; WHILE ... (double ;) *)
-(** In a traditional functional programming language like OCaml or
-    Haskell we could add the [WHILE] case as follows:
-
-  Fixpoint ceval_fun (st : state) (c : com) : state :=
-    match c with
-      ...
-      | WHILE b DO c END =>
-          if (eval st b)
-            then ceval_fun st (c; WHILE b DO c END)
-            else st
-    end.
-*)
-  
